work on impl some more

disk-betree/ImplFlushPolicy.i.dfy
@@ -1,17 +1,19 @@
-include "ImplModelFlush.i.dfy"
-include "ImplModelGrow.i.dfy"
-include "ImplModelSplit.i.dfy"
-include "ImplModelLeaf.i.dfy"
-include "Bounds.i.dfy"
+include "ImplFlush.i.dfy"
+include "ImplGrow.i.dfy"
+include "ImplSplit.i.dfy"
+include "ImplLeaf.i.dfy"
+include "ImplModelFlushPolicy.i.dfy"
 
-module ImplModelFlushPolicy {
-  import opened ImplModel
-  import opened ImplModelIO
-  import opened ImplModelCache
-  import opened ImplModelFlush
-  import opened ImplModelGrow
-  import opened ImplModelSplit
-  import opened ImplModelLeaf
+module ImplFlushPolicy {
+  import opened Impl
+  import opened ImplIO
+  import opened ImplCache
+  import opened ImplFlush
+  import opened ImplGrow
+  import opened ImplSplit
+  import opened ImplLeaf
+  import ImplModelFlushPolicy
+  import opened ImplState
 
   import opened Sequences
 
@@ -21,138 +23,74 @@ module ImplModelFlushPolicy {
   import opened BucketWeights
   import KMTable
 
-  datatype Action =
-    | ActionPageIn(ref: BT.G.Reference)
-    | ActionSplit(parentref: BT.G.Reference, slot: uint64)
-    | ActionFlush(parentref: BT.G.Reference, slot: uint64)
-    | ActionRepivot(ref: BT.G.Reference)
-    | ActionGrow
-    | ActionEvict
-    | ActionFail
-
-  function biggestSlotIterate(buckets: seq<KMTable.KMTable>, j: uint64, bestIdx: uint64, bestWeight: uint64) : (res : (uint64, uint64))
-  requires 0 <= bestIdx as int < |buckets|
-  requires 0 <= bestWeight as int <= MaxTotalBucketWeight()
-  requires 1 <= j as int <= |buckets| <= MaxNumChildren()
-  requires forall i | 0 <= i < |buckets| :: |buckets[i].keys| == |buckets[i].values|
-  requires WeightBucketList(KMTable.ISeq(buckets)) <= MaxTotalBucketWeight()
-  requires WeightBucket(KMTable.I(buckets[bestIdx])) == bestWeight as int
-  ensures 0 <= res.0 as int < |buckets|
-  ensures 0 <= res.1 as int <= MaxTotalBucketWeight()
-  ensures WeightBucket(KMTable.I(buckets[res.0])) == res.1 as int
-  decreases |buckets| - j as int
-  {
-    if j == |buckets| as uint64 then (
-      (bestIdx, bestWeight)
-    ) else (
-      WeightBucketLeBucketList(KMTable.ISeq(buckets), j as int);
-
-      var w := WeightBucket(KMTable.I(buckets[j])) as uint64;
-      if w > bestWeight then (
-        biggestSlotIterate(buckets, j+1, j, w)
-      ) else (
-        biggestSlotIterate(buckets, j+1, bestIdx, bestWeight)
-      )
-    )
-  }
-
-  function biggestSlot(buckets: seq<KMTable.KMTable>) : (res : (uint64, uint64))
-  requires |buckets| > 0
-  requires |buckets| <= MaxNumChildren()
-  requires forall i | 0 <= i < |buckets| :: |buckets[i].keys| == |buckets[i].values|
-  requires WeightBucketList(KMTable.ISeq(buckets)) <= MaxTotalBucketWeight()
-  ensures 0 <= res.0 as int < |buckets|
-  ensures 0 <= res.1 as int <= MaxTotalBucketWeight()
-  ensures WeightBucket(KMTable.I(buckets[res.0])) == res.1 as int
+  method biggestSlot(buckets: seq<KMTable.KMTable>) returns (res : (uint64, uint64))
+  requires forall i | 0 <= i < |buckets| :: KMTable.WF(buckets[i])
+  requires ImplModelFlushPolicy.biggestSlot.requires(buckets)
+  ensures res == ImplModelFlushPolicy.biggestSlot(buckets)
   {
     WeightBucketLeBucketList(KMTable.ISeq(buckets), 0);
-    biggestSlotIterate(buckets, 1, 0, WeightBucket(KMTable.I(buckets[0])) as uint64)
+    KMTable.kmtableWeightEq(buckets[0]);
+    var j := 1;
+    var bestIdx := 0;
+    var bestWeight := KMTable.computeWeightKMTable(buckets[0]);
+    while j < |buckets| as uint64
+    invariant ImplModelFlushPolicy.biggestSlotIterate.requires(buckets, j, bestIdx, bestWeight)
+    invariant ImplModelFlushPolicy.biggestSlotIterate(buckets, j, bestIdx, bestWeight) == ImplModelFlushPolicy.biggestSlot(buckets)
+    {
+      KMTable.kmtableWeightEq(buckets[j]);
+      WeightBucketLeBucketList(KMTable.ISeq(buckets), j as int);
+      var w := KMTable.computeWeightKMTable(buckets[j]);
+      if w > bestWeight {
+        bestIdx := j;
+        bestWeight := w;
+      }
+      j := j + 1;
+    }
+
+    return (bestIdx, bestWeight);
   }
 
-  predicate ValidStackSlots(k: Constants, s: Variables, stack: seq<BT.G.Reference>, slots: seq<uint64>)
-  {
-    && |stack| == |slots| + 1
-    && s.Ready?
-    && (forall j | 0 <= j < |stack| :: stack[j] in s.cache)
-    && (forall j | 0 <= j < |stack| - 1 :: s.cache[stack[j]].children.Some?)
-    && (forall j | 0 <= j < |stack| - 1 :: slots[j] as int < |s.cache[stack[j]].children.value| <= MaxNumChildren())
-    && (forall j | 0 <= j < |stack| - 1 :: slots[j] as int < |s.cache[stack[j]].children.value| <= MaxNumChildren())
-  }
-
-  predicate ValidAction(k: Constants, s: Variables, action: Action)
-  {
-    && s.Ready?
-    && (action.ActionPageIn? ==> (
-      && action.ref in s.ephemeralIndirectionTable
-      && action.ref !in s.cache
-      && s.ephemeralIndirectionTable[action.ref].0.Some?
-    ))
-    && ((action.ActionSplit? || action.ActionFlush?) ==> (
-      && action.parentref in s.ephemeralIndirectionTable
-      && action.parentref in s.cache
-      && s.cache[action.parentref].children.Some?
-      && 0 <= action.slot as int < |s.cache[action.parentref].children.value|
-      && s.cache[action.parentref].children.value[action.slot] in s.cache
-      && s.cache[action.parentref].children.value[action.slot] in s.ephemeralIndirectionTable
-    ))
-    && (action.ActionSplit? ==> (
-      && |s.cache[s.cache[action.parentref].children.value[action.slot]].buckets| >= 2
-      && |s.cache[action.parentref].buckets| <= MaxNumChildren() - 1
-    ))
-    && (action.ActionRepivot? ==> (
-      && action.ref != BT.G.Root()
-      && action.ref in s.ephemeralIndirectionTable
-      && action.ref in s.cache
-      && s.cache[action.ref].children.None?
-    ))
-  }
-
-  function method getActionToPageIn(cache: map<BT.G.Reference, Node>, ref: BT.G.Reference) : Action
-  {
-    // TODO eviction
-    /*
-    if |cache| >= MaxCacheSize() then
-      ActionEvict
-    else*/
-      ActionPageIn(ref)
-  }
-
-  function {:opaque} getActionToSplit(k: Constants, s: Variables, stack: seq<BT.G.Reference>, slots: seq<uint64>, i: uint64) : (action : Action)
+  method getActionToSplit(k: ImplConstants, s: ImplVariables, stack: seq<BT.G.Reference>, slots: seq<uint64>, i: uint64) returns (action : ImplModelFlushPolicy.Action)
   requires 0 <= i as int < |stack|
-  requires WFVars(s)
-  requires ValidStackSlots(k, s, stack, slots)
+  requires Inv(k, s)
+  requires ImplModelFlushPolicy.ValidStackSlots(Ic(k), IVars(s), stack, slots)
+  ensures action == ImplModelFlushPolicy.getActionToSplit(Ic(k), IVars(s), stack, slots, i)
   {
-    if i == 0 then
+    ImplModelFlushPolicy.reveal_getActionToSplit();
+
+    if i == 0 {
       // Can't split root until we grow it.
-      ActionGrow
-    else (
-      if |s.cache[stack[i-1]].children.value| as uint64 < MaxNumChildren() as uint64 then (
-        if |s.cache[stack[i]].buckets| as uint64 == 1 then (
-          ActionRepivot(stack[i])
-        ) else (
-          ActionSplit(stack[i-1], slots[i-1])
-        )
-      ) else (
-        getActionToSplit(k, s, stack, slots, i-1)
-      )
-    )
+      action := ImplModelFlushPolicy.ActionGrow;
+    } else {
+      if |s.cache[stack[i-1]].children.value| as uint64 < MaxNumChildren() as uint64 {
+        if |s.cache[stack[i]].buckets| as uint64 == 1 {
+          action := ImplModelFlushPolicy.ActionRepivot(stack[i]);
+        } else {
+          action := ImplModelFlushPolicy.ActionSplit(stack[i-1], slots[i-1]);
+        }
+      } else {
+        action := getActionToSplit(k, s, stack, slots, i-1);
+      }
+    }
   }
 
-  function {:opaque} getActionToFlush(k: Constants, s: Variables, stack: seq<BT.G.Reference>, slots: seq<uint64>) : (action : Action)
+  method getActionToFlush(k: ImplConstants, s: ImplVariables, stack: seq<BT.G.Reference>, slots: seq<uint64>) returns (action : ImplModelFlushPolicy.Action)
   requires |stack| <= 40
-  requires ValidStackSlots(k, s, stack, slots)
-  requires WFVars(s)
+  requires ImplModelFlushPolicy.ValidStackSlots(Ic(k), IVars(s), stack, slots)
+  requires Inv(k, s)
   decreases 0x1_0000_0000_0000_0000 - |stack|
+  ensures action == ImplModelFlushPolicy.getActionToFlush(Ic(k), IVars(s), stack, slots)
   {
-    if |stack| as uint64 == 40 then (
-      ActionFail
-    ) else (
+    if |stack| as uint64 == 40 {
+      action := ImplModelFlushPolicy.ActionFail;
+    } else {
       var ref := stack[|stack| as uint64 - 1];
       var node := s.cache[ref];
-      if node.children.None? || |node.buckets| == MaxNumChildren() then (
-        getActionToSplit(k, s, stack, slots, |stack| as uint64 - 1)
-      ) else (
-        var (slot, slotWeight) := biggestSlot(node.buckets);
+      if node.children.None? || |node.buckets| == MaxNumChildren() {
+        action := getActionToSplit(k, s, stack, slots, |stack| as uint64 - 1);
+      } else {
+        var bs := biggestSlot(node.buckets);
+        var (slot, slotWeight) := bs;
         // TODO partial flushes
         // with partial flushes, we can ensure that the node will either have a lot of children
         // or will have a flushable node.
@@ -160,25 +98,35 @@ module ImplModelFlushPolicy {
 
         //if slotWeight >= FlushTriggerWeight() as uint64 then (
           var childref := node.children.value[slot];
-          if childref in s.cache then (
+          if childref in s.cache {
             var child := s.cache[childref];
-            var childTotalWeight: uint64 := WeightBucketList(KMTable.ISeq(child.buckets)) as uint64;
-            var extraRootWeight: uint64 := if ref == BT.G.Root() then WeightBucket(s.rootBucket) as uint64 else 0;
-            if slotWeight + childTotalWeight + extraRootWeight <= MaxTotalBucketWeight() as uint64 then (
-              ActionFlush(ref, slot)
-            ) else (
-              getActionToFlush(k, s, stack + [childref], slots + [slot])
-            )
-          ) else (
-            getActionToPageIn(s.cache, childref)
-          )
+
+            KMTable.kmtableSeqWeightEq(child.buckets);
+            var childTotalWeight: uint64 := KMTable.computeWeightKMTableSeq(child.buckets);
+
+            var extraRootWeight: uint64;
+            if ref == BT.G.Root() {
+              extraRootWeight := WeightBucket(s.rootBucket);
+            } else {
+              extraRootWeight := 0;
+            }
+
+            if slotWeight + childTotalWeight + extraRootWeight <= MaxTotalBucketWeight() as uint64 {
+              action := ImplModelFlushPolicy.ActionFlush(ref, slot);
+            } else {
+              action := ImplModelFlushPolicy.getActionToFlush(k, s, stack + [childref], slots + [slot]);
+            }
+          } else {
+            action := ImplModelFlushPolicy.getActionToPageIn(s.cache, childref);
+          }
         //) else (
         //  getActionToSplit(k, s, stack, slots, |stack| as uint64 - 1)
         //)
-      )
-    )
+      }
+    }
   }
 
+  /*
   lemma getActionToSplitValidAction(k: Constants, s: Variables, stack: seq<BT.G.Reference>, slots: seq<uint64>, i: uint64)
   requires 0 <= i as int < |stack|
   requires Inv(k, s)
@@ -400,4 +348,5 @@ module ImplModelFlushPolicy {
       }
     }
   }
+  */
 }
